Finish proof of safety of Stenning

fairneris/examples/stenning_code.v
@@ -81,28 +81,30 @@ Definition mBA_in (n : Z) (S: gset message) : Prop :=
   ∃ msg, msg ∈ S ∧ good_message false n (Some msg).
 
 Definition client_RT (n : Z) (R T : gset message) : Prop :=
-  (∀ m, mBA_in m R → mAB_in m T) ∧
+  (∀ m, mBA_in m R → (m >= 0)%Z → mAB_in m T) ∧
   (∀ m, m >= n → ¬ mBA_in m R)%Z.
 
 Definition server_RT (n : Z) (R T : gset message) : Prop :=
-  (∀ m, mBA_in m R → mAB_in m T) ∧
-  (∀ m, m >= n → ¬ mBA_in m R)%Z.
+  (∀ m, 0 <= m → mBA_in m T → mAB_in m R)%Z ∧
+  (∀ m, 0 <= m → m ≤ n → (mBA m) ∈ T)%Z ∧
+  (∀ m, m > n → ¬ mAB_in m R)%Z.
 
-Definition garbage_message b msg := ∀ m, ¬ good_message b m (Some msg).
+Definition garbage_message b msg := ∀ m, (m >= 0)%Z → ¬ good_message b m (Some msg).
 
 Lemma client_RT_good msg n R T :
+  (n >= 0)%Z →
   good_message false n (Some msg) →
   client_RT n R T →
   client_RT (n + 1) ({[msg]} ∪ R) ({[ mAB n ]} ∪ T).
 Proof.
-  intros Hg (HRT & Hnin). split_and!.
-  - intros m [msgm [[Hin%elem_of_singleton | Hin]%elem_of_union Hgoodm]].
+  intros Hn Hg (HRT & Hnin). split_and!.
+  - intros m [msgm [[Hin%elem_of_singleton | Hin]%elem_of_union Hgoodm]] Hm.
     + simplify_eq.
       have -> : n = m by eapply good_message_inj.
       exists (mAB m). split; [set_solver|]. exists (mAB m). split_and!; try naive_solver. simpl.
       rewrite ZOfString_inv //.
     + have [x [??]] : mAB_in m T.
-      * apply HRT. by exists msgm.
+      * apply HRT =>//. by exists msgm.
       * exists x. naive_solver set_solver.
   - intros m Hm [msg' [[Hin%elem_of_singleton | Hin]%elem_of_union ?]].
     + simplify_eq. have ? : n = m by eapply good_message_inj. lia.
@@ -110,36 +112,119 @@ Proof.
 Qed.
 
 Lemma client_RT_garbage n G R T :
+  (n >= 0)%Z →
   (∀ msg, msg ∈ G → garbage_message false msg) →
   client_RT n R T →
   client_RT n (G ∪ R) ({[ mAB n ]} ∪ T).
 Proof.
-  intros Hgar (HRT & Hnin). split_and!.
-  - intros m [msgm [[Hin | Hin]%elem_of_union Hgoodm]].
-    + exfalso. eapply (Hgar msgm Hin m Hgoodm).
+  intros Hn Hgar (HRT & Hnin). split_and!.
+  - intros m [msgm [[Hin | Hin]%elem_of_union Hgoodm]] Hm.
+    + exfalso. unshelve eapply (Hgar msgm Hin m _ Hgoodm). lia.
     + have [x [??]] : mAB_in m T.
-      * apply HRT. by exists msgm.
+      * apply HRT=>//. by exists msgm.
       * exists x. naive_solver set_solver.
   - intros m Hm [msgm [[Hin | Hin]%elem_of_union Hgoodm]].
-    + exfalso. eapply (Hgar msgm Hin m Hgoodm).
+    + unshelve eapply (Hgar msgm Hin m _ Hgoodm). lia.
     + ospecialize (Hnin m _). lia. apply Hnin. exists msgm. naive_solver.
 Qed.
 
 Lemma client_RT_garbage_emp n R T :
+  (n >= 0)%Z →
   client_RT n R T →
   client_RT n R ({[ mAB n ]} ∪ T).
 Proof.
   pose proof (client_RT_garbage n ∅ R T) as Hccl.
   replace (∅ ∪ R) with R in Hccl by set_solver.
-  intros ?. apply Hccl=>//.
+  intros ??. apply Hccl=>//.
 Qed.
 
 Lemma client_RT_garbage_singleton n msg R T :
+  (n >= 0)%Z →
   (garbage_message false msg) →
   client_RT n R T →
   client_RT n ({[ msg ]} ∪ R) ({[ mAB n ]} ∪ T).
 Proof.
   intros **. eapply client_RT_garbage=>//. naive_solver set_solver.
+Qed.
+
+Lemma server_RT_good msg n R T :
+  good_message true n (Some msg) →
+  server_RT (n-1)%Z R T →
+  server_RT n ({[msg]} ∪ R) ({[ mBA n ]} ∪ T).
+Proof.
+  intros Hgood HRT. split_and!.
+  - intros m Hm0 [msgm [[-> % elem_of_singleton | Hin]%elem_of_union Hgoodm]] .
+    + have ?: n = m.
+      { destruct Hgoodm as (?&Ha&Hb&Hc). simplify_eq. rewrite /mBA /= ZOfString_inv in Hb. naive_solver. }
+      simplify_eq. exists msg. naive_solver set_solver.
+    + have [x [??]] : mAB_in m R.
+      * apply HRT =>//. by exists msgm.
+      * exists x. naive_solver set_solver.
+  - intros m Hm0 Hmn. destruct (decide (m = n)).
+    + simplify_eq. by apply elem_of_union; left; apply elem_of_singleton.
+    + apply elem_of_union; right. apply HRT; lia.
+  - intros m Hmn (msg'&Hin&Hgood'). apply elem_of_union in Hin; destruct Hin as [Hin|Hin].
+    + apply elem_of_singleton in Hin; simplify_eq. have: m = n; last lia.
+      eapply good_message_inj=>//.
+    + destruct HRT as (?&?&Hnin). unshelve eapply (Hnin m _). lia. by exists msg'.
+Qed.
+
+Lemma server_RT_garbage_1 msg n R T :
+  (n >= -1)%Z →
+  (garbage_message true msg) →
+  server_RT n R T →
+  server_RT n ({[msg]} ∪ R) ({[ mBA n ]} ∪ T).
+Proof.
+  intros Nn0 Hgar HRT. destruct HRT as (Hincl&Hin'&Hnin). split_and!.
+  - intros m Hm0 [msgm [[Hin%elem_of_singleton | Hin]%elem_of_union Hgoodm]].
+    + simplify_eq. have ?: n = m.
+      { destruct Hgoodm as (?&Ha&Hb&Hc). simplify_eq. rewrite /mBA /= ZOfString_inv in Hb. naive_solver. }
+      simplify_eq. have ? := Hm0. apply (Hin' m) in Hm0 =>//.
+      have [msgin ?] : mAB_in m R.
+      { apply Hincl=>//. exists (mBA m). naive_solver. }
+      exists msgin. naive_solver set_solver.
+    + have Hinp: mBA_in m T.
+      { exists msgm. naive_solver. }
+      apply Hincl in Hinp as [msgin ?]=>//. exists msgin. naive_solver set_solver.
+  - intros m Hm0 Hmn. destruct (decide (m = n)).
+    + simplify_eq. by apply elem_of_union; left; apply elem_of_singleton.
+    + apply elem_of_union; right. apply Hin'; lia.
+  - intros m Hmn (msg'&Hin&Hgood'). apply elem_of_union in Hin; destruct Hin as [Hin|Hin].
+    + apply elem_of_singleton in Hin; simplify_eq. apply (Hgar m). lia. done.
+    + unshelve eapply (Hnin m _). lia. by exists msg'.
+Qed.
+
+Lemma server_RT_garbage_2 msg n R T :
+  (n >= -1)%Z →
+  (garbage_message true msg) →
+  server_RT n R T →
+  server_RT n ({[msg]} ∪ R) T.
+Proof.
+  intros Nn0 Hgar HRT. destruct HRT as (Hincl&Hin'&Hnin). split_and!.
+  - intros m Hm0 [msgm [Hin Hgood]].
+    + have Hinp: mBA_in m T.
+      { exists msgm. naive_solver. }
+      apply Hincl in Hinp as [msgin ?]=>//. exists msgin. naive_solver set_solver.
+  - intros m Hm0 Hmn. apply Hin'=>//.
+  - intros m Hmn (msg'&Hin&Hgood'). apply elem_of_union in Hin; destruct Hin as [Hin|Hin].
+    + apply elem_of_singleton in Hin; simplify_eq. apply (Hgar m). lia. done.
+    + unshelve eapply (Hnin m _). lia. by exists msg'.
+Qed.
+
+Lemma server_RT_garbage_3 msg n R T :
+  (n >= -1)%Z →
+  (garbage_message false msg) →
+  server_RT n R T →
+  server_RT n R ({[msg]} ∪ T).
+Proof.
+  intros Nn0 Hgar HRT. destruct HRT as (Hincl&Hin'&Hnin). split_and!.
+  - intros m Hm0 [msgm [[Hin%elem_of_singleton | Hin]%elem_of_union Hgoodm]].
+    + simplify_eq. exfalso. apply (Hgar m)=>//. lia.
+    + have Hinp: mBA_in m T.
+      { exists msgm. naive_solver. }
+      apply Hincl in Hinp as [msgin ?]=>//. exists msgin. naive_solver set_solver.
+  - intros m Hm0 Hmn. apply elem_of_union; right. apply Hin'=>//.
+  - intros m Hmn (msg'&Hin&Hgood'). unshelve eapply (Hnin m _). lia. by exists msg'.
 Qed.
 
 Section with_Σ.
@@ -158,7 +243,7 @@ Section with_Σ.
 
   Definition retinv : iProp Σ := frag_free_roles_are ∅ ∗
      ∃ stA stB, frag_model_is (stA, stB) ∗ own stenning_A_name (●E stA) ∗ own stenning_B_name (●E stB) ∗
-      let (n, m) := stenning_get_n (stA, stB) in ⌜ (n = m ∨ n = m + 1)%Z ⌝ ∗ saA ↦c{1/4} n ∗ saB ↦c{1/4} m.
+      let (n, m) := stenning_get_n (stA, stB) in ⌜ (n = m ∨ m = n + 1)%Z ⌝ ∗ saA ↦c{1/4} n ∗ saB ↦c{1/4} (m-1)%Z.
 
   Lemma token_update γ {A: ofe} {_: inG Σ (excl_authR A)} (st st' st'' : A) :
     own γ (●E st) ∗ own γ (◯E st'') ==∗ own γ (●E st') ∗ own γ (◯E st').
@@ -179,9 +264,7 @@ Section with_Σ.
 
   Definition client_si (m : message) : iProp Σ :=
     ∃ (n : Z), ⌜ m_body m = StringOfZ n ⌝ ∗
-         saA ↦c{1/4} n ∗
-         saB ↦c{1/4} n
-  .
+         (⌜ n >= 0 ⌝%Z → saA ↦c{1/4} n ∗ saB ↦c{1/4} n).
 
   Definition server_si (m : message) : iProp Σ :=
     ∃ (n : Z), ⌜ m_body m = StringOfZ n ⌝ ∗
@@ -298,13 +381,16 @@ Section with_Σ.
 
       iSpecialize ("Hnew" with "[]").
       { naive_solver. }
-      iDestruct "Hnew" as (j) "(%Hbody' & Hcc' & Hcs)".
+      iDestruct "Hnew" as (j) "(%Hbody' & Hnew)".
+      iDestruct ("Hnew" with "[]") as "(Hcc' & Hcs)".
+      { destruct Hgood as (?&Hcount&?). simplify_eq. rewrite Hbody' ZOfString_inv in Hcount.
+        simplify_eq. iPureIntro; lia. }
+
       iDestruct (lmapsto_agree with "Hcc' Hcc") as %->.
       iDestruct (lmapsto_agree with "Hcs Hcsi") as %Hcseq.
 
       iCombine "Hcc Hcci Hcc'" as "Hcc".
-      replace (1/2 + (1/4 + 1/4))%Qp with 1%Qp; last first.
-      { admit. (* Q reasonning *) }
+      replace (1/2 + (1/4 + 1/4))%Qp with 1%Qp by compute_done.
       iDestruct (gen_heap_light_update (L:=socket_address) _ _ _ _ (n+1)%Z
              with "Hw Hcc") as ">[Hw [Hcc [Hccm Hcci]]]".
 
@@ -320,9 +406,9 @@ Section with_Σ.
       iMod ("Hclose'" with "[Hw]"); first naive_solver.
       iMod ("Hclose" with "[Hfr Hmod HstA HstB Hcci Hcsi]").
       { iNext. rewrite /retinv. iFrame. iExists (ASending (1+n)), _. iFrame.
-        rewrite /stenning_get_n /= -Hcseq. iSplit.
-        * iPureIntro. right. lia.
-        * rewrite Z.add_comm. admit. (* Qp reasonning. *) }
+        rewrite /stenning_get_n /=. iSplit.
+        * iPureIntro. simplify_eq. left. lia.
+        * rewrite Z.add_comm. replace (1/2/2)%Qp with (1/4)%Qp by compute_done. iFrame. }
       iModIntro. iApply wp_value'. do 5 wp_pure _.
       clear Hcseq.
       simplify_eq. rewrite bool_decide_true; last by do 2 f_equal.
@@ -334,7 +420,8 @@ Section with_Σ.
       { rewrite Z.add_comm //. }
       { iPureIntro; lia. }
       { iPureIntro. apply client_RT_good=>//. exists msg. naive_solver. }
-      { iIntros. replace (n + 1 - 1)%Z with n by lia. iFrame. admit. (* Qp *) }
+      { iIntros. replace (n + 1 - 1)%Z with n by lia. iFrame.
+        replace (1/2/2)%Qp with (1/4)%Qp by compute_done. iFrame. }
     - iApply (mu_step_model _ _ _ _ ∅ ∅ _ ((ASending n, stB) : stenning_model) with "Hmod [Hf] [Hfr //]").
       { simpl. by apply A_RecvFail. }
       { set_solver. }
@@ -376,30 +463,40 @@ Section with_Σ.
         { intros Hc. simplify_eq. apply Hbad. eexists; split=>//. }
         rewrite bool_decide_false //; last naive_solver. wp_pure _.
 
-        iAssert (⌜ msg ∈ R ⌝)%I with "[Hnew Hcc]" as %Hin.
-        { destruct (decide (msg ∈ R)) as [|Hnin]=>//. iSpecialize ("Hnew" $! Hnin).
-          rewrite /client_si.
-          iDestruct "Hnew" as (n') "(%Hbody & Hcc' & _)".
-          iDestruct (lmapsto_agree with "Hcc' Hcc") as %->.
-          rewrite Hbody ZOfString_inv in Heqmsg. simplify_eq. }
+        destruct (decide (msg_n >= 0)%Z).
 
-        iApply ("IH" with "[] [$Hst] [$] [$Hsh] [] [$HRT] [] [] [$Hcc] [$Hf]").
-        { iPureIntro; lia. }
-        { iPureIntro; lia. }
-        { iPureIntro. replace ({[msg]} ∪ R) with R by set_solver.
-          apply client_RT_garbage_emp=>//. }
-        { iIntros (Hnin). exfalso. apply Hnin. set_solver. }
-  Admitted.
+        * iAssert (⌜ msg ∈ R ⌝)%I with "[Hnew Hcc]" as %Hin.
+          { destruct (decide (msg ∈ R)) as [|Hnin]=>//. iSpecialize ("Hnew" $! Hnin).
+            rewrite /client_si.
+            iDestruct "Hnew" as (j) "(%Hbody' & Hnew)".
+            iDestruct ("Hnew" with "[]") as "(Hcc' & Hcs)".
+            { simplify_eq. rewrite Hbody' ZOfString_inv in Heqmsg. simplify_eq. iPureIntro; lia. }
+                iDestruct (lmapsto_agree with "Hcc' Hcc") as %->.
+            rewrite Hbody' ZOfString_inv in Heqmsg. simplify_eq. }
+
+          iApply ("IH" with "[] [$Hst] [$] [$Hsh] [] [$HRT] [] [] [$Hcc] [$Hf]").
+          { iPureIntro; lia. }
+          { iPureIntro; lia. }
+          { iPureIntro. replace ({[msg]} ∪ R) with R by set_solver.
+            apply client_RT_garbage_emp=>//. }
+          { iIntros (Hnin). exfalso. apply Hnin. set_solver. }
+        * iApply ("IH" with "[] [$Hst] [$] [$Hsh] [] [$HRT] [] [] [$Hcc] [$Hf]").
+          { iPureIntro; lia. }
+          { iPureIntro; lia. }
+          { iPureIntro. apply client_RT_garbage_singleton=>//. intros ??.
+            intros (?&?&?&?&?). simplify_eq. }
+          { iIntros. exfalso. set_solver. }
+  Qed.
 
   Lemma wp_server tid (f : nat) (Hf: f > 40) :
-    {{{ inv Ns retinv ∗ is_node ipB ∗ saA ⤇ (λ msg, ⌜ msg = msg⌝) ∗ saB ⤇ (λ msg, ⌜ msg = msg⌝) ∗
-          own stenning_B_name (◯E (BReceiving 0)) ∗
+    {{{ inv Ns retinv ∗ counter_inv ∗ is_node ipB ∗ saA ⤇ client_si ∗ saB ⤇ server_si ∗
+          own stenning_B_name (◯E (BReceiving 0)) ∗ saB ↦c{1/2} (-1)%Z ∗
           (ipB, tid) ↦M {[ Brole := f ]} ∗ saB ⤳ (∅, ∅) ∗
           free_ports (ip_of_address saB) {[port_of_address saB]} }}}
       (mkExpr (ip_of_address saB) (server saA saB #())) @ (ipB, tid); ⊤
     {{{ v, RET v; (ipB, tid) ↦M ∅ }}}.
   Proof.
-    iIntros (Φ) "(#Hinv&#Hin&#HsA&#HsB&Hst&Hf&HRT&Hfp) HΦ".
+    iIntros (Φ) "(#Hinv&#Hcinv&#Hin&#HsA&#HsB&Hst&Hcs&Hf&HRT&Hfp) HΦ".
     rewrite /server.
     wp_pure _.
 
@@ -429,24 +526,29 @@ Section with_Σ.
     { iExists _. iFrame. iPureIntro. lia. }
     clear f Hf.
 
-    iAssert (∃ R T, saB ⤳ (R, T))%I with "[HRT]" as (R T) "HRT".
-    { iExists _, _. iFrame. }
-
-    remember (-1) as n eqn:Heq.
+    remember (-1)%Z as n eqn:Heq.
     replace (BReceiving 0) with (BReceiving (1+n)); last naive_solver.
 
-    assert (n >= -1) as Hn; first lia. clear Heq.
-    iLöb as "IH" forall (f' n Hn R T) "Hf". iDestruct "Hf'" as %Hf.
+    iAssert (∃ R T, saB ⤳ (R, T) ∗ ⌜ server_RT n R T ⌝)%I
+      with "[HRT]" as (R T) "(HRT & HinvRT)".
+    { iExists _, _. iFrame. rewrite /server_RT. iPureIntro.
+      split_and!; naive_solver (set_solver || lia). }
+
+    assert (n >= -1)%Z as Hn; first lia. clear Heq.
+    iLöb as "IH" forall (f' n Hn R T) "Hf". iDestruct "Hf'" as %Hf. iDestruct "HinvRT" as %HinvRT.
 
     wp_pure _.
 
     wp_bind (ReceiveFrom _).
     iApply sswp_MU_wp_fupd.
-    iInv Ns as "Hi" "Hclose". iModIntro.
+    iInv Ns as "Hi" "Hclose". iInv Nc as "Hw" "Hclose'". iModIntro.
 
     iApply (wp_recv with "[Hsh] [HRT] [HsA]")=>//=>//=>//.
-    iNext. iDestruct "Hi" as "(Hfr & %stA & %stB & Hmod & HstA & HstB & %Hnm)".
+    iNext. iDestruct "Hi" as "(Hfr & %stA & %stB & Hmod & HstA & HstB & Hcounters)".
     iDestruct (token_agree with "HstB Hst") as %->.
+
+    rewrite /stenning_get_n /=. iDestruct "Hcounters" as "(%Hcrel & Hcci & Hcsi)".
+    iDestruct "Hw" as (w) "Hw".
 
     iIntros (om r) "Hmsg".
 
@@ -465,26 +567,54 @@ Section with_Σ.
       { rewrite fmap_empty map_union_empty. done. }
       iIntros "Hmod Hf Hfr".
       rewrite map_union_empty /usr_fl /=.
+
+      iDestruct (lmapsto_agree with "Hcsi Hcs") as %->.
+
+      iDestruct ("Hnew" with "[]") as (msg_n Hmsgbody) "[Hccm Hcsm]".
+      { iPureIntro. destruct HinvRT as (?&?&Hnin). intros Hc.
+        eapply (Hnin (1+n)%Z). lia. eexists. split=>//. exists msg'. naive_solver. }
+
+      iDestruct (lmapsto_agree with "Hcs Hcsm") as %Hcseq. simplify_eq.
+      replace (1 + (msg_n - 1))%Z with msg_n by lia.
+      iDestruct (lmapsto_agree with "Hcci Hccm") as %Hcseq.
+
+      iCombine "Hcs Hcsi Hcsm" as "Hcs".
+      replace (1/2 + (1/4 + 1/4))%Qp with 1%Qp by compute_done.
+      iDestruct (gen_heap_light_update (L:=socket_address) _ _ _ _ msg_n
+             with "Hw Hcs") as ">[Hw [Hcs [Hcsm Hcsi]]]".
+
       iMod (token_update with "[$HstB $Hst]") as "[HstB Hst]".
-      iMod ("Hclose" with "[Hfr Hmod HstA HstB]").
-      { iNext. rewrite /retinv. iFrame. iExists _, _. iFrame. admit. }
+      iMod ("Hclose'" with "[Hw]"); first naive_solver.
+      iMod ("Hclose" with "[Hfr Hmod HstA HstB Hcsi Hcci]").
+      { iNext. rewrite /retinv. iFrame. iExists _, _. cbn. iFrame. cbn.
+        replace (1 + msg_n - 1)%Z with msg_n by lia; cbn.
+        replace (1 / 2 / 2)%Qp with (1/4)%Qp by compute_done. iFrame.
+        iPureIntro. rewrite !Hcseq. lia. }
+
       iModIntro. iApply wp_value'. do 5 wp_pure _.
       rewrite bool_decide_true; last by do 2 f_equal.
       do 3 wp_pure _.
       { simpl. rewrite Hbody //. }
-      do 5 wp_pure _. rewrite bool_decide_true //. do 3 wp_pure _.
+      do 5 wp_pure _. rewrite bool_decide_true //; last by (do 3 f_equal; lia). do 3 wp_pure _.
 
       wp_bind (SendTo _ _ _).
       iApply sswp_MU_wp_fupd.
 
       iInv Ns as "Hi" "Hclose". iModIntro.
-      iApply (wp_send _ _ false with "[Hsh] [HRT] [HsB]")=>//=>//=>//.
-      iNext. iIntros "Hsh HRT". clear Hnm stA.
-      iDestruct "Hi" as "(Hfr & %stA & %stB & Hmod & HstA & HstB & Hnm)".
-      iDestruct (token_agree with "HstB Hst") as %->.
+      iApply (wp_send _ _ false with "[Hsh] [HRT] [HsB] [Hcsm Hccm]")=>//=>//=>//.
+      { iNext. iExists msg_n. iFrame.
+        replace (1 / 2 / 2)%Qp with (1/4)%Qp by compute_done. iFrame. iPureIntro. cbn.
+        split. f_equal; lia. lia. }
 
-      iApply (mu_step_model _ _ _ _ ∅ ∅ _ ((stA, (BReceiving (1+(1+n)))) : stenning_model) with "Hmod [Hf] [Hfr //]").
-      { simpl. replace (Send _) with (Send (mBA $ (1 + (1 + n)) - 1)). constructor. f_equal.
+      iNext. iIntros "Hsh HRT". clear Hcrel Hcseq stA.
+      iDestruct "Hi" as "(Hfr & %stA & %stB & Hmod & HstA & HstB & Hcounters)".
+      iDestruct (token_agree with "HstB Hst") as %->.
+      rewrite /stenning_get_n /=. iDestruct "Hcounters" as "(%Hcrel & Hcci & Hcsi)".
+      iDestruct (lmapsto_agree with "Hcsi Hcs") as %->.
+
+      iApply (mu_step_model _ _ _ _ ∅ ∅ _ ((stA, (BReceiving (1 + msg_n)))%Z : stenning_model) with "Hmod [Hf] [Hfr //]").
+      { simpl.
+        replace (Send _) with (Send (mBA ((1 + msg_n) - 1)))%Z. constructor. f_equal.
         rewrite /mBA //=. do 2 f_equal. lia. }
       { set_solver. }
       { set_solver. }
@@ -492,12 +622,17 @@ Section with_Σ.
       iIntros "Hmod Hf Hfr".
 
       iMod (token_update with "[$HstB $Hst]") as "[HstB Hst]".
-      iMod ("Hclose" with "[Hfr Hmod HstA HstB]").
-      { iNext. rewrite /retinv. iFrame. iExists _, _. iFrame. admit. }
+      iMod ("Hclose" with "[Hfr Hmod HstA HstB Hcci Hcsi]").
+      { iNext. rewrite /retinv. iFrame. iExists _, _. iFrame. cbn.
+        replace (1 + msg_n - 1)%Z with msg_n by lia. iFrame. iPureIntro. naive_solver. }
       rewrite map_union_empty /usr_fl /=. iModIntro. iApply wp_value'. do 3 wp_pure _.
-      iApply ("IH" with "[] [Hst] [$] [$] [] [$HRT] [$]")=>//.
+      iApply ("IH" with "[] [Hst] [Hcs] [$HΦ] [$Hsh] [] [$HRT] [] [$Hf]")=>//.
       { iPureIntro; lia. }
-      { rewrite Z.add_comm //. }
+      { replace (1 + (1 + (msg_n - 1)))%Z with (1 + msg_n)%Z by lia. iFrame. }
+      { replace (1 + (msg_n - 1))%Z with msg_n by lia. iFrame. }
+      { iPureIntro. lia. }
+      { iPureIntro. replace (1 + (msg_n - 1))%Z with msg_n by lia.
+        apply server_RT_good=>//. exists msg'. rewrite Hmsgbody ZOfString_inv. naive_solver. }
     - iApply (mu_step_model _ _ _ _ ∅ ∅ _ ((stA, BReceiving (1+n)) : stenning_model) with "Hmod [Hf] [Hfr //]").
       { simpl. by apply B_RecvFailEmpty. }
       { set_solver. }
@@ -505,13 +640,19 @@ Section with_Σ.
       { rewrite fmap_empty map_union_empty. done. }
       iIntros "Hmod Hf Hfr".
       rewrite map_union_empty /usr_fl /=.
-      iMod ("Hclose" with "[Hfr Hmod HstA HstB]").
-      { iNext. rewrite /retinv. iFrame. iExists _, _. iFrame. admit. }
+      iMod ("Hclose'" with "[Hw]"); first by naive_solver.
+      iDestruct (lmapsto_agree with "Hcsi Hcs") as %Heq.
+      iMod ("Hclose" with "[Hfr Hmod HstA HstB Hcsi Hcci]").
+      { iNext. rewrite /retinv. iFrame. iExists _, _. iFrame. cbn. iFrame. iPureIntro. naive_solver. }
       iModIntro. iApply wp_value'.
-      iDestruct "Hmsg" as "[(-> & %Heq & Hsh & HRT)|(%msg' & -> & %Heq & %Heqdest & Hsh & HRT & Hnew)]".
-      + do 3 wp_pure _. iApply ("IH" with "[] [Hst] [$] [$] [] [$HRT] [$]")=>//.
+      iDestruct "Hmsg" as "[(-> & %Heq' & Hsh & HRT)|(%msg' & -> & %Heq' & %Heqdest & Hsh & HRT & Hnew)]".
+      + do 3 wp_pure _.
+        iApply ("IH" with "[] [Hst] [Hcs] [$HΦ] [$Hsh] [] [$HRT] [] [$Hf]")=>//.
+        { iPureIntro; lia. }
       + do 5 wp_pure _. rewrite bool_decide_false; last naive_solver.
-        wp_pure _. iApply ("IH" with "[] [Hst] [$] [$] [] [$HRT] [$]")=>//.
+        wp_pure _. iApply ("IH" with "[] [Hst] [Hcs] [$HΦ] [$Hsh] [] [$HRT] [] [$Hf]")=>//.
+        { iPureIntro; lia. }
+        { iPureIntro. apply server_RT_garbage_2=>//. intros ??(?&?&?&?&?). naive_solver. }
     - iDestruct "Hmsg" as "[(-> & %Heq & Hsh & HRT)|(%msg' & -> & %Heq & %Heqdest & Hsh & HRT & Hnew)]".
       { simplify_eq. naive_solver. }
       simplify_eq. have ?: m_sender msg' = saA by apply NNP_P; naive_solver.
@@ -523,48 +664,80 @@ Section with_Σ.
       iIntros "Hmod Hf Hfr".
       rewrite map_union_empty /usr_fl /=.
       iMod (token_update with "[$HstB $Hst]") as "[HstB Hst]".
-      iMod ("Hclose" with "[Hfr Hmod HstA HstB]").
-      { iNext. rewrite /retinv. iFrame. iExists _, _. iFrame. admit. }
+      iMod ("Hclose'" with "[Hw]"); first by naive_solver.
+      iDestruct (lmapsto_agree with "Hcsi Hcs") as %Heq.
+      iMod ("Hclose" with "[Hfr Hmod HstA HstB Hcsi Hcci]").
+      { iNext. rewrite /retinv. iFrame. iExists _, _. iFrame. cbn. iFrame. iPureIntro. naive_solver. }
       iModIntro. iApply wp_value'. do 5 wp_pure _. rewrite bool_decide_true; last by do 2 f_equal.
-      destruct (ZOfString (m_body msg')) as [?|] eqn:Heq.
-      + do 3 wp_pure _; first by rewrite /= Heq. do 5 wp_pure _. rewrite bool_decide_false; last first.
+      destruct (ZOfString (m_body msg')) as [msg_n|] eqn:Heq'.
+      + do 3 wp_pure _; first by rewrite /= Heq'. do 5 wp_pure _. rewrite bool_decide_false; last first.
         { intros ?; simplify_eq. apply Hbad. rewrite /good_message Z.add_comm //. naive_solver. }
         do 2 wp_pure _. wp_bind (SendTo _ _ _).
         iApply sswp_MU_wp_fupd. iInv Ns as "Hi" "Hclose". iModIntro.
-        iApply (wp_send _ _ false with "[Hsh] [HRT] [HsB]")=>//=>//=>//.
-        iNext. iIntros "Hsh HRT". clear Hnm stA.
-        iDestruct "Hi" as "(Hfr & %stA & %stB & Hmod & HstA & HstB & Hnm)".
+        iApply (wp_send _ _ (if decide (n >= 0)%Z then true else false) with "[Hsh] [HRT] [HsB]")=>//=>//=>//.
+        { destruct (decide _).
+          - iPureIntro. destruct HinvRT as (?&HT&?). ospecialize (HT n _ _). lia. lia. naive_solver.
+          - iNext. iExists n. cbn. iSplit=>//. by iIntros. }
+        iNext. iIntros "Hsh HRT". clear Hcrel stA.
+        iDestruct "Hi" as "(Hfr & %stA & %stB & Hmod & HstA & HstB & Hcounters)".
+        rewrite /stenning_get_n /=. iDestruct "Hcounters" as "(%Hcrel & Hcci & Hcsi)".
+        iDestruct (lmapsto_agree with "Hcsi Hcs") as %->.
         iDestruct (token_agree with "HstB Hst") as %->.
-        iApply (mu_step_model _ _ _ _ ∅ ∅ _ ((stA, (BReceiving (1+n))) : stenning_model) with "Hmod [Hf] [Hfr //]").
-        { simpl. replace (Send _) with (Send (mBA $ (1 + n) - 1)). constructor. f_equal.
+        iApply (mu_step_model _ _ _ _ ∅ ∅ _ ((stA, (BReceiving (1+n))) : stenning_model)
+                 with "Hmod [Hf] [Hfr //]").
+        { simpl. replace (Send _) with (Send (mBA $ (1 + n) - 1))%Z. constructor. f_equal.
           rewrite /mBA //=. do 2 f_equal. lia. }
         { set_solver. }
         { set_solver. }
         { rewrite fmap_empty map_union_empty. done. }
         iIntros "Hmod Hf Hfr".
         iMod (token_update with "[$HstB $Hst]") as "[HstB Hst]".
-        iMod ("Hclose" with "[Hfr Hmod HstA HstB]").
-        { iNext. rewrite /retinv. iFrame. iExists _, _. iFrame. admit. }
+        iMod ("Hclose" with "[Hfr Hmod HstA HstB Hcci Hcsi]").
+        { iNext. rewrite /retinv. iFrame. iExists _, _. iFrame. cbn.
+          replace (1 + n - 1)%Z with n. iFrame. iPureIntro. naive_solver. }
         rewrite map_union_empty /usr_fl /=. iModIntro. iApply wp_value'. do 2 wp_pure _.
-        iApply ("IH" with "[] [Hst] [$] [$] [] [$HRT] [$]")=>//.
-      + do 3 wp_pure _; first by rewrite /= Heq. do 7 wp_pure _.
+
+        destruct (decide (msg' ∈ R)) as [|Hnin].
+        * iApply ("IH" with "[] [Hst] [Hcs] [$HΦ] [$Hsh] [] [$HRT] [] [$Hf]")=>//.
+          { iPureIntro; lia. }
+          { iPureIntro. destruct HinvRT as (?&HR&?).
+            replace ({[msg']} ∪ R) with R by set_solver.
+            destruct (decide (n < 0)%Z).
+            + apply server_RT_garbage_3=>//. intros ??(?&?&?&?&?). simpl in *. simplify_eq. simpl in *.
+              rewrite ->ZOfString_inv in *. simplify_eq. naive_solver.
+            + opose proof (HR n _ _); try lia. replace (_ ∪ T) with T by set_solver. split_and!=>//. }
+        * iSpecialize ("Hnew" $! Hnin).
+          rewrite /server_si.
+          iDestruct "Hnew" as (j) "(%Hbody' & Hccm & Hcsm)".
+          iDestruct (lmapsto_agree with "Hcs Hcsm") as %->.
+          rewrite Hbody' ZOfString_inv in Heq'. simplify_eq.
+          exfalso. apply Hbad. exists msg'. split_and!=>//. rewrite Hbody' ZOfString_inv. f_equal. lia.
+      + do 3 wp_pure _; first by rewrite /= Heq'. do 7 wp_pure _.
         wp_bind (SendTo _ _ _).
         iApply sswp_MU_wp_fupd. iInv Ns as "Hi" "Hclose". iModIntro.
-        iApply (wp_send _ _ false with "[Hsh] [HRT] [HsB]")=>//=>//=>//.
-        iNext. iIntros "Hsh HRT". clear Hnm stA.
-        iDestruct "Hi" as "(Hfr & %stA & %stB & Hmod & HstA & HstB & %Hnm)".
+        iApply (wp_send _ _ (if decide (n >= 0)%Z then true else false) with "[Hsh] [HRT] [HsB]")=>//=>//=>//.
+        { destruct (decide _).
+          - iPureIntro. destruct HinvRT as (?&HT&?). ospecialize (HT n _ _). lia. lia. naive_solver.
+          - iNext. iExists n. cbn. iSplit=>//. by iIntros. }
+        iNext. iIntros "Hsh HRT". clear Hcrel stA.
+        iDestruct "Hi" as "(Hfr & %stA & %stB & Hmod & HstA & HstB & Hcounters)".
+        rewrite /stenning_get_n /=. iDestruct "Hcounters" as "(%Hcrel & Hcci & Hcsi)".
+        iDestruct (lmapsto_agree with "Hcsi Hcs") as %->.
         iDestruct (token_agree with "HstB Hst") as %->.
         iApply (mu_step_model _ _ _ _ ∅ ∅ _ ((stA, (BReceiving (1+n))) : stenning_model) with "Hmod [Hf] [Hfr //]").
-        { simpl. replace (Send _) with (Send (mBA $ (1 + n) - 1)). constructor. f_equal.
+        { simpl. replace (Send _) with (Send (mBA $ (1 + n) - 1))%Z. constructor. f_equal.
           rewrite /mBA //=. do 2 f_equal. lia. }
         { set_solver. }
         { set_solver. }
         { rewrite fmap_empty map_union_empty. done. }
         iIntros "Hmod Hf Hfr".
         iMod (token_update with "[$HstB $Hst]") as "[HstB Hst]".
-        iMod ("Hclose" with "[Hfr Hmod HstA HstB]").
-        { iNext. rewrite /retinv. iFrame. iExists _, _. iFrame. admit. }
+        iMod ("Hclose" with "[Hfr Hmod HstA HstB Hcci Hcsi]").
+        { iNext. rewrite /retinv. iFrame. iExists _, _. iFrame. cbn.
+          replace (1 + n - 1)%Z with n. iFrame. iPureIntro. naive_solver. }
         rewrite map_union_empty /usr_fl /=. iModIntro. iApply wp_value'. do 2 wp_pure _.
-        iApply ("IH" with "[] [Hst] [$] [$] [] [$HRT] [$]")=>//.
-  Admitted.
+        iApply ("IH" with "[] [Hst] [Hcs] [$HΦ] [$Hsh] [] [$HRT] [] [$Hf]")=>//.
+        { iPureIntro; lia. }
+        { iPureIntro. apply server_RT_garbage_1=>//. intros ??(?&?&?&?). naive_solver. }
+  Qed.
 End with_Σ.
